cedar-dafny/pe/soundness.dfy
@@ -2,7 +2,9 @@ include "def.dfy"
 include "environment.dfy"
 include "engine.dfy"
 include "../def/core.dfy"
+include "../def/base.dfy"
 include "../def/engine.dfy"
+include "../def/std.dfy"
 
 module pe.soundness {
   import opened definition
@@ -10,6 +12,23 @@ module pe.soundness {
   import opened engine
   import ce = def.engine
   import def.core
+  import def.base
+  import opened def.std
+
+  lemma makeErrorValueIsErr(env: Environment)
+    requires env.wellFormed()
+    ensures var r := PartialEvaluator.makeErrorValue(); env.interpret(r, core.EntityStore(map[])).Err? {
+      calc {
+        env.interpret(PartialEvaluator.makeErrorValue(), core.EntityStore(map[]));
+        ==
+        calc {
+          env.interpret(Residual.Record([]), core.EntityStore(map[]));
+          ==
+          Ok(core.Value.Record(map[]));
+        }
+        Err(base.AttrDoesNotExist);
+      }
+    }
 
   lemma PEIsSound(e: definition.Expr, q: core.Request, s: core.EntityStore, Q: definition.Request, S: definition.EntityStore, env: Environment)
     requires env.wellFormed()
@@ -17,7 +36,13 @@ module pe.soundness {
     requires var ps := env.replaceUnknownInEntityStore(S); ps.Some? && ps.value == s
     ensures var peRes := PartialEvaluator(Q, S).interpret(e);
             // If PE succeeds, then evaluating the residual and evaluating the original expression with the same unknown to value mappings should agree.
-            (peRes.Ok? ==> ce.Evaluator(q, s).interpret(env.replaceUnknownInExpr(e)) == env.interpret(peRes.value)) &&
+            (peRes.Ok? ==> ce.Evaluator(q, s).interpret(env.replaceUnknownInExpr(e)) == env.interpret(peRes.value, s)) &&
             // If PE fails, then evaluating the original expression with any uknown to value mappings should fail.
             (peRes.Err? ==> ce.Evaluator(q, s).interpret(env.replaceUnknownInExpr(e)).Err?)
+  {
+    match e {
+      case PrimitiveLit(_) =>
+      case _ => assume false;
+    }
+  }
 }
